WIP

src/Experiments/FancyMachineMontgomery256.v
@@ -6,1136 +6,120 @@ Require Import Crypto.BoundedArithmetic.ArchitectureToZLikeProofs.
 Require Import Crypto.ModularArithmetic.Montgomery.ZBounded.
 Require Import Crypto.ModularArithmetic.Montgomery.ZProofs.
 Require Import Crypto.Util.Tuple Crypto.Util.Option Crypto.Util.Sigma Crypto.Util.Prod.
-(* These might be needed for faster lookups *)
-(*Require Import Coq.FSets.FMaps Coq.FSets.FMapAVL Coq.FSets.FMapFacts Coq.FSets.FMapFullAVL.*)
-
-Require Import Bedrock.Word.
-Require Import Crypto.Util.GlobalSettings.
-Require Import Crypto.Util.Tactics.
-Require Import Crypto.Util.Notations.
-Require Import Crypto.Tactics.VerdiTactics.
-Require Import Coq.ZArith.BinInt.
-Require Import Coq.Lists.List.
-
-Require Import Crypto.Assembly.Evaluables.
+Require Import Crypto.Reflection.Syntax.
+Require Import Crypto.Reflection.Linearize.
+Require Import Crypto.Reflection.CommonSubexpressionElimination.
+Require Import Crypto.Reflection.Reify.
 
 Local Open Scope Z_scope.
 Notation eta x := (fst x, snd x).
 Notation eta3 x := (eta (fst x), snd x).
 Notation eta3' x := (fst x, eta (snd x)).
 
-Section fold.
-  Context {A B} (f : A -> B) (join : B -> B -> B).
-  Fixpoint tuple'_fold {n : nat} : tuple' A n -> B
-    := match n with
-       | 0%nat => fun v => f v
-       | S n' => fun v => join (tuple'_fold (fst v)) (f (snd v))
-       end.
-
-  Definition tuple_fold (init : B) {n : nat} : tuple A n -> B
-    := match n with
-       | 0%nat => fun v => init
-       | S n' => tuple'_fold
-       end.
-End fold.
-
-Axiom (modulus : Z) (m' : Z) (Hm : modulus <> 0) (H : 0 <= modulus < 2^256) (Hm' : 0 <= m' < 2^256) (ops : fancy_machine.instructions (2 * 128)) (props : fancy_machine.arithmetic ops).
-Let H' : 0 <= 256 <= 256. omega. Qed.
-Let H'' : 0 < 256. omega. Qed.
-Let props' := ZLikeProperties_of_ArchitectureBoundedOps ops modulus H 256 H' H''.
-Let ops' := (ZLikeOps_of_ArchitectureBoundedOps ops modulus 256).
-Let fst' := @fst fancy_machine.W fancy_machine.W.
-Let snd' := @snd fancy_machine.W fancy_machine.W.
-Let ldi : load_immediate
-            (@ZBounded.SmallT (2 ^ 256) (2 ^ 256) modulus
-                              (@ZLikeOps_of_ArchitectureBoundedOps 128 ops modulus 256)) := _.
-Let isldi : is_load_immediate ldi := _.
-Let f := (fun v => proj1_sig (reduce_via_partial (2^256) modulus (props := props') (ldi m') I Hm (fst' v, snd' v))).
-
-Section Definitions.
-  Inductive vartype := Tbool | TW.
-  Inductive consttype := TZ | Tvar (_ : vartype).
-  Inductive flat_type := Tconst (_ : consttype) | Prod (_ _ : flat_type).
-  Inductive type := Tflat (_ : flat_type) | Arrow : vartype -> type -> type.
-  Global Coercion Tvar : vartype >-> consttype.
-  Global Coercion Tconst : consttype >-> flat_type.
-  Global Coercion Tflat : flat_type >-> type.
-
-  Fixpoint interp_flat_type (t:flat_type): Type :=
-    match t with
-    | Prod a b => prod (interp_flat_type a) (interp_flat_type b)
-    | TZ => Z
-    | TW => fancy_machine.W
-    | Tbool => bool
-    end.
-
-  Fixpoint interp_type (t:type): Type :=
-    match t with
-    | Arrow a b => interp_flat_type a -> interp_type b
-    | Tflat t => interp_flat_type t
-    end.
-
-  Section ind.
-    Local Notation TZ := (Tconst TZ).
-    Local Notation TW := (Tconst TW).
-    Local Notation Tbool := (Tconst Tbool).
-    Inductive nop : forall (narg nret : nat), tuple flat_type narg -> tuple flat_type nret -> Type :=
-    | OPldi     : nop 1 1 TZ TW
-    | OPshrd    : nop 3 1 (TW, TW, TZ) TW
-    | OPshl     : nop 2 1 (TW, TZ) TW
-    | OPshr     : nop 2 1 (TW, TZ) TW
-    | OPmkl     : nop 2 1 (TW, TZ) TW
-    | OPadc     : nop 3 2 (TW, TW, Tbool) (Tbool, TW)
-    | OPsubc    : nop 3 2 (TW, TW, Tbool) (Tbool, TW)
-    | OPmulhwll : nop 2 1 (TW, TW) TW
-    | OPmulhwhl : nop 2 1 (TW, TW) TW
-    | OPmulhwhh : nop 2 1 (TW, TW) TW
-    | OPselc    : nop 3 1 (Tbool, TW, TW) TW
-    | OPaddm    : nop 3 1 (TW, TW, TW) TW.
-  End ind.
-
-  Definition interp_nop {narg nret t1 t2} (op:@nop narg nret t1 t2)
-    : tuple_fold interp_flat_type prod unit t1
-      -> tuple_fold interp_flat_type prod unit t2
-    := match op in (@nop narg nret t1 t2)
-             return tuple_fold interp_flat_type prod unit t1
-                    -> tuple_fold interp_flat_type prod unit t2
-       with
-       | OPldi => fun args => ldi args
-       | OPshrd => fun args => let '(x1, x2, x3) := eta3 args in shrd x1 x2 x3
-       | OPshl => fun args => let '(x1, x2) := eta args in shl x1 x2
-       | OPshr => fun args => let '(x1, x2) := eta args in shr x1 x2
-       | OPmkl => fun args => let '(x1, x2) := eta args in mkl x1 x2
-       | OPadc => fun args => let '(x1, x2, x3) := eta3 args in adc x1 x2 x3
-       | OPsubc => fun args => let '(x1, x2, x3) := eta3 args in subc x1 x2 x3
-       | OPmulhwll => fun args => let '(x1, x2) := eta args in mulhwll x1 x2
-       | OPmulhwhl => fun args => let '(x1, x2) := eta args in mulhwhl x1 x2
-       | OPmulhwhh => fun args => let '(x1, x2) := eta args in mulhwhh x1 x2
-       | OPselc => fun args => let '(x1, x2, x3) := eta3 args in selc x1 x2 x3
-       | OPaddm => fun args => let '(x1, x2, x3) := eta3 args in addm x1 x2 x3
-       end.
-End Definitions.
-
-Inductive SpecialZConst : Set := Cmodulus | Cm'.
-Fixpoint interp_SpecialZConst (e: SpecialZConst) : Z :=
-  match e with Cmodulus => modulus | Cm' => m' end.
-
-Module Input.
-  Section Language.
-    Section expr.
-      Context {var : flat_type -> Type}.
-
-      Inductive expr : type -> Type :=
-      | Const : forall {t : flat_type}, interp_type t -> expr t
-      | SpZConst : SpecialZConst -> expr TZ
-      | Var : forall {t}, var t -> expr t
-      | Unop : forall {t1 t2}, @nop 1 1 t1 t2
-                               -> expr t1 -> expr (tuple_fold id Prod TZ t2)
-      | Binop : forall {t10 t11 t2}, @nop 2 1 (t10, t11) t2
-                                     -> expr t10 -> expr t11 -> expr (tuple_fold id Prod TZ t2)
-      | Trinop : forall {t10 t11 t12 t2}, @nop 3 1 (t10, t11, t12) t2
-                                          -> expr t10 -> expr t11 -> expr t12 -> expr (tuple_fold id Prod TZ t2)
-      | Trinop2Ret : forall {t10 t11 t12 t2}, @nop 3 2 (t10, t11, t12) t2
-                                              -> expr t10 -> expr t11 -> expr t12 -> expr (tuple_fold id Prod TZ t2)
-      | Let : forall {tx : flat_type}, expr tx -> forall {tC}, (var tx -> expr tC) -> expr tC
-      | Pair : forall {t1 : flat_type}, expr t1 -> forall {t2 : flat_type}, expr t2 -> expr (Prod t1 t2)
-      | Abs : forall {t1 : vartype} {t2}, (var t1 -> expr t2) -> expr (Arrow t1 t2)
-      | MatchPair : forall {t1 t2}, expr (Prod t1 t2) -> forall {tC}, (var t1 -> var t2 -> expr tC) -> expr tC.
-    End expr.
-
-    Definition Expr t : Type := forall var, @expr var t.
-
-    Fixpoint interp {t} (e: @expr interp_type t) : interp_type t :=
-      match e in @expr _ t return interp_type t with
-      | Const _ n => n
-      | SpZConst n => interp_SpecialZConst n
-      | Var _ n => n
-      | Unop _ _ op e1 => interp_nop op (interp e1)
-      | Binop _ _ _ op e1 e2 => interp_nop op (interp e1, interp e2)
-      | Trinop _ _ _ _ op e1 e2 e3 => interp_nop op (interp e1, interp e2, interp e3)
-      | Trinop2Ret _ _ _ _ op e1 e2 e3 => interp_nop op (interp e1, interp e2, interp e3)
-      | Let _ ex _ eC => let x := interp ex in interp (eC x)
-      | Pair _ e1 _ e2 => (interp e1, interp e2)
-      | Abs _ _ f => fun x => interp (f x)
-      | MatchPair _ _ ep _ eC => let (v1, v2) := interp ep in interp (eC v1 v2)
-      end.
-
-    Definition Interp {t} (E:Expr t) : interp_type t := interp (E interp_type).
-  End Language.
-
-  (* Reification assumes the argument type is Z *)
-
-  Ltac reify_type t :=
-    lazymatch t with
-    | BinInt.Z => TZ
-    | bool => Tbool
-    | fancy_machine.W => TW
-    | prod ?l ?r =>
-      let l := reify_type l in
-      let r := reify_type r in
-      constr:(Prod l r)
-    | ?l -> ?r =>
-      let l := reify_type l in
-      let r := reify_type r in
-      constr:(Arrow l r)
-    end.
-
-  Ltac reify_nop op :=
-    lazymatch op with
-    | @Interface.ldi     => OPldi
-    | @Interface.shrd    => OPshrd
-    | @Interface.shl     => OPshl
-    | @Interface.shr     => OPshr
-    | @Interface.mkl     => OPmkl
-    | @Interface.adc     => OPadc
-    | @Interface.subc    => OPsubc
-    | @Interface.mulhwll => OPmulhwll
-    | @Interface.mulhwhl => OPmulhwhl
-    | @Interface.mulhwhh => OPmulhwhh
-    | @Interface.selc    => OPselc
-    | @Interface.addm    => OPaddm
-    end.
-
-  Class reify {varT} (var:varT) {eT} (e:eT) {T:Type} := Build_reify : T.
-  Definition reify_var_for_in_is {T} (x:T) (t:flat_type) {eT} (e:eT) := False.
-
-  Class absify {eT} (e:eT) {T:Type} := Build_absify : T.
-
-  Ltac reify var e :=
-    lazymatch e with
-    | let x := ?ex in @?eC x =>
-      let ex := reify var ex in
-      let eC := reify var eC in
-      constr:(Let (var:=var) ex eC)
-    | match ?ep with (v1, v2) => @?eC v1 v2 end =>
-      let ep := reify var ep in
-      let eC := reify var eC in
-      constr:(MatchPair (var:=var) ep eC)
-    | pair ?a ?b =>
-      let a := reify var a in
-      let b := reify var b in
-      constr:(Pair (var:=var) a b)
-    | (fun x : ?T => ?C) =>
-      let t := reify_type T in
-      (* Work around Coq 8.5 and 8.6 bug *)
-      (* <https://coq.inria.fr/bugs/show_bug.cgi?id=4998> *)
-      (* Avoid re-binding the Gallina variable referenced by Ltac [x] *)
-      (* even if its Gallina name matches a Ltac in this tactic. *)
-      let maybe_x := fresh x in
-      let not_x := fresh x in
-      let C := lazymatch constr:(fun (x : T) (not_x : var t) (_:reify_var_for_in_is x t not_x) =>
-                                   (_ : reify var C)) (* [C] here is an open term that references "x" by name *)
-               with fun _ v _ => @?C v => C end in
-      C
-    | modulus => constr:(SpZConst (var := var) Cmodulus)
-    | m' => constr:(SpZConst (var := var) Cm')
-    | ?x
-      => lazymatch goal with
-         | _:reify_var_for_in_is x ?t ?v |- _ => constr:(@Var var t v)
-         | _
-           => let op := head x in
-              let op := match x with
-                        | _ => reify_nop op
-                        | _ => let t := (let t := type of x in reify_type t) in
-                               constr:(@Const var t x)
-                        end in
-              lazymatch op with
-              | @Const _ _ _ => op
-              | _
-                => let op := match constr:(Set) with
-                             | _ => constr:(Unop (var:=var) op)
-                             | _ => constr:(Binop (var:=var) op)
-                             | _ => constr:(Trinop (var:=var) op)
-                             | _ => constr:(Trinop2Ret (var:=var) op)
-                             end in
-                   lazymatch op with
-                   | Unop _ => lazymatch x with
-                               | ?op' ?a
-                                 => let a := reify var a in
-                                    constr:(op a)
-                               end
-                   | Binop _ => lazymatch x with
-                                | ?op' ?a ?b
-                                  => let a := reify var a in
-                                     let b := reify var b in
-                                     constr:(op a b)
-                                end
-                   | Trinop _ => lazymatch x with
-                                 | ?op' ?a ?b ?c
-                                   => let a := reify var a in
-                                      let b := reify var b in
-                                      let c := reify var c in
-                                      constr:(op a b c)
-                                 end
-                   | Trinop2Ret _ => lazymatch x with
-                                     | ?op' ?a ?b ?c
-                                       => let a := reify var a in
-                                          let b := reify var b in
-                                          let c := reify var c in
-                                          constr:(op a b c)
-                                     end
-                   end
-              end
-         end
-    end.
-  Local Ltac idtac_goal := match goal with |- ?G => idtac "Goal:" G end.
-  Hint Extern 0 (reify ?var ?e) => (let e := reify var e in eexact e) : typeclass_instances.
-
-  Ltac Reify e :=
-    lazymatch constr:(fun (var:flat_type->Type) => (_:reify var e)) with
-      (fun var => ?C) => constr:(fun (var:flat_type->Type) => C) (* copy the term but not the type cast *)
-    end.
-
-  Definition example_expr var : expr (var:=var) (Arrow TW (Arrow TW TW)).
-  Proof.
-    let f' := (eval cbv [f] in (fun x y => f (x, y))) in
-    let f' := (eval simpl in f') in
-    let f' := (eval unfold fst', snd', fst, snd in f') in
-    let rv := reify var f' in
-    let rv := constr:(Abs (fun x => Abs (fun y => rv x y))) in
-    let rv := (eval cbv beta in rv) in
-    exact rv.
-  Defined.
-
-  Definition example_Expr : Expr (Arrow TW (Arrow TW TW))
-    := example_expr.
-
-  Lemma example_expr_good : interp (@example_expr _) = (fun x y => f (x, y)).
-  Proof.
-    cbv [Interp interp example_expr fst snd interp_nop].
-    unfold f; simpl.
-    reflexivity.
-  Qed.
-
-  Lemma example_Expr_good : Interp example_Expr = (fun x y => f (x, y)).
-  Proof.
-    apply example_expr_good.
-  Qed.
-
-  Ltac lhs_of_goal := match goal with |- ?R ?LHS ?RHS => constr:(LHS) end.
-  Ltac rhs_of_goal := match goal with |- ?R ?LHS ?RHS => constr:(RHS) end.
-
-  (*Ltac Reify_rhs :=
-    let rhs := rhs_of_goal in
-    let RHS := Reify rhs in
-    transitivity (ZInterp RHS);
-    [|cbv iota beta delta [ZInterp Interp interp_type interp_binop interp]; reflexivity].
-
-  Goal (0 = let x := 1+2 in x*3)%Z.
-    Reify_rhs.
-  Abort.
-
-  Goal (0 = let x := 1 in let y := 2 in x * y)%Z.
-    Reify_rhs.
-  Abort.*)
-
-  Section wf.
-    Context {var1 var2 : flat_type -> Type}.
-
-    Local Notation "x ≡ y" := (existT _ _ (x, y)).
-
-    Inductive wf : list (sigT (fun t => var1 t * var2 t))%type -> forall {t}, @expr var1 t -> @expr var2 t -> Prop :=
-    | WfConst : forall G t n, wf G (Const (t := t) n) (Const n)
-    | WfSpZConst : forall G n, wf G (SpZConst n) (SpZConst n)
-    | WfVar : forall G (t : flat_type) x x', In (x ≡ x') G -> @wf G t (Var x) (Var x')
-    | WfUnop : forall G {t1 t2} (op : nop 1 1 t1 t2) (e1:@expr var1 t1) (e1':@expr var2 t1),
-        wf G e1 e1'
-        -> wf G (Unop op e1) (Unop op e1')
-    | WfBinop : forall G {t10 t11 t2} (op : nop 2 1 (t10, t11) t2)
-                       (e10:@expr var1 t10) (e11:@expr var1 t11)
-                       (e10':@expr var2 t10) (e11':@expr var2 t11),
-        wf G e10 e10'
-        -> wf G e11 e11'
-        -> wf G (Binop op e10 e11) (Binop op e10' e11')
-    | WfTrinop : forall G {t10 t11 t12 t2} (op : nop 3 1 (t10, t11, t12) t2)
-                       (e10:@expr var1 t10) (e11:@expr var1 t11) (e12:@expr var1 t12)
-                       (e10':@expr var2 t10) (e11':@expr var2 t11) (e12':@expr var2 t12),
-        wf G e10 e10'
-        -> wf G e11 e11'
-        -> wf G e12 e12'
-        -> wf G (Trinop op e10 e11 e12) (Trinop op e10' e11' e12')
-    | WfTrinop2Ret : forall G {t10 t11 t12 t2} (op : nop 3 2 (t10, t11, t12) t2)
-                       (e10:@expr var1 t10) (e11:@expr var1 t11) (e12:@expr var1 t12)
-                       (e10':@expr var2 t10) (e11':@expr var2 t11) (e12':@expr var2 t12),
-        wf G e10 e10'
-        -> wf G e11 e11'
-        -> wf G e12 e12'
-        -> wf G (Trinop2Ret op e10 e11 e12) (Trinop2Ret op e10' e11' e12')
-    | WfLet : forall G t1 t2 e1 e1' (e2 : _ t1 -> @expr _ t2) e2',
-        wf G e1 e1'
-        -> (forall x1 x2, wf ((x1 ≡ x2) :: G) (e2 x1) (e2' x2))
-        -> wf G (Let e1 e2) (Let e1' e2')
-    | WfAbs : forall G t1 t2 e e',
-        (forall x1 x2, wf ((x1 ≡ x2) :: G) (e x1) (e' x2))
-        -> wf G (@Abs _ t1 t2 e) (Abs e')
-    | WfPair : forall G {t1 t2 : flat_type} (e1: @expr var1 t1) (e2: @expr var1 t2)
-                      (e1': @expr var2 t1) (e2': @expr var2 t2),
-        wf G e1 e1'
-        -> wf G e2 e2'
-        -> wf G (Pair e1 e2) (Pair e1' e2')
-    | WfMatchPair : forall G t1 t2 tC ep ep' (eC : _ t1 -> _ t2 -> @expr _ tC) eC',
-        wf G ep ep'
-        -> (forall x1 x2 y1 y2, wf ((x1 ≡ x2) :: (y1 ≡ y2) :: G) (eC x1 y1) (eC' x2 y2))
-        -> wf G (MatchPair ep eC) (MatchPair ep' eC').
-  End wf.
-
-  Definition Wf {t} (E : @Expr t) := forall var1 var2, wf nil (E var1) (E var2).
-
-  Example example_Expr_Wf : Wf example_Expr.
-  Proof.
-    repeat match goal with
-           | [ |- Wf _ ] => unfold Wf; intros
-           | [ |- wf _ _ _ ] => constructor
-           | [ |- In ?x (cons ?x _) ] => constructor 1; reflexivity
-           | [ |- In _ _ ] => progress unfold tuple'_fold, id, fst, snd
-           | [ |- In ?x (cons _ ?xs) ]
-             => match xs with context[x] => constructor 2 end
-           | _ => intros
-           end.
-  Qed.
-
-  (*Axiom Wf_admitted : forall {t} (E:Expr t), @Wf Z t E.
-  Ltac admit_Wf := apply Wf_admitted.*)
-End Input.
-
-Module Output.
-
-  Section Language.
-    (* A very restricted language where binary operations are restricted
-    to returning [T] and must appear in [let] binders, and all pairs
-    must be constructed in the return clause.  No matching on pairs is
-    allowed *)
-
-    Section expr.
-      Context {var : vartype -> Type}.
-
-      Inductive arg : flat_type -> Type :=
-      | Const {t} : @interp_type (Tconst t) -> arg t
-      | SpZConst : SpecialZConst -> arg TZ
-      | Var {t} : var t -> arg t
-      | Pair : forall {t1}, arg t1 -> forall {t2}, arg t2 -> arg (Prod t1 t2).
-
-      Inductive expr : type -> Type :=
-      | LetUnop : forall {t1}, nop 1 1 t1 TW -> arg t1 ->
-                               forall {tC}, (var TW -> expr tC) -> expr tC
-      | LetBinop : forall {t1 t2}, nop 2 1 (t1, t2) TW -> arg t1 -> arg t2 ->
-                                   forall {tC}, (var TW -> expr tC) -> expr tC
-      | LetTrinop : forall {t1 t2 t3}, nop 3 1 (t1, t2, t3) TW -> arg t1 -> arg t2 -> arg t3 ->
-                                       forall {tC}, (var TW -> expr tC) -> expr tC
-      | LetTrinop2Ret : forall {t1 t2 t3}, nop 3 2 (t1, t2, t3) (Tconst Tbool, Tconst TW)
-                                           -> arg t1 -> arg t2 -> arg t3 ->
-                                           forall {tC}, (var Tbool -> var TW -> expr tC) -> expr tC
-      | Abs : forall {t1 : vartype} {t2}, (var t1 -> expr t2) -> expr (Arrow t1 t2)
-      | Return : forall {t}, arg t -> expr t.
-    End expr.
-
-    Arguments arg _ _ : clear implicits.
-    Arguments expr _ _ : clear implicits.
-
-    Definition Expr t : Type := forall var, expr var t.
-
-    Fixpoint simple_arg_type (t : type) : flat_type
-      := match t with
-         | Arrow _ t => simple_arg_type t
-         | Tflat t => t
-         end.
-    Fixpoint under_arrows (t1 : type) (tf : flat_type -> type) :=
-      match t1 with
-      | Arrow s d => Arrow s (under_arrows d tf)
-      | Tflat t => tf t
-      end.
-    Definition simple_arg {var} t := @arg var (simple_arg_type t).
-    Arguments simple_arg _ _ : clear implicits.
-    Coercion simple_arg_of_arg {var t} (x : arg var t) : simple_arg var t
-      := x.
-
-    Fixpoint interp_arg {t} (e: arg interp_type t) : interp_type t :=
-      match e with
-      | Const _ n => n
-      | SpZConst n => interp_SpecialZConst n
-      | Var _ n => n
-      | Pair _ e1 _ e2 => (interp_arg e1, interp_arg e2)
-      end.
-
-    Fixpoint interp {t} (e:expr interp_type t) : interp_type t :=
-      match e with
-      | LetUnop _ op a _ eC
-        => let x := interp_nop op (interp_arg a) in interp (eC x)
-      | LetBinop _ _ op a b _ eC
-        => let x := interp_nop op (interp_arg a, interp_arg b) in interp (eC x)
-      | LetTrinop _ _ _ op a b c _ eC
-        => let x := interp_nop op (interp_arg a, interp_arg b, interp_arg c) in interp (eC x)
-      | LetTrinop2Ret _ _ _ op a b c _ eC
-        => let '(c, v) := eta (interp_nop op (interp_arg a, interp_arg b, interp_arg c)) in interp (eC c v)
-      | Abs _ _ f => fun x => @interp _ (f x)
-      | Return _ a => interp_arg a
-      end.
-
-    Definition Interp {t} (E:Expr t) : interp_type t := interp (E interp_type).
-  End Language.
-
-  Section arg_map.
-    Fixpoint map_arg {var1 var2} (f : forall x, var1 x -> var2 x) {t} (v : @arg var1 t) : @arg var2 t
-      := match v in @arg _ t return @arg _ t with
-         | Const _ x => Const x
-         | SpZConst x => SpZConst x
-         | Var _ v => Var (f _ v)
-         | Pair _ x _ y => Pair (map_arg f x) (map_arg f y)
-         end.
-  End arg_map.
-
-  Section under_lets.
-    Context {var: vartype -> Type}.
-
-    Arguments arg _ _ : clear implicits.
-    Arguments simple_arg _ _ : clear implicits.
-    Arguments expr _ _ : clear implicits.
-
-    Fixpoint under_lets {t} (e: expr var t) {struct e} :
-      forall {tC} (C:simple_arg var t -> expr var tC), expr var (under_arrows t (fun _ => tC))
-      := match e in (expr _ t) return forall {tC} (C:simple_arg var t -> expr var tC), expr var (under_arrows t (fun _ => tC)) with
-         | LetUnop _ op a _ eC
-           => fun tC C => LetUnop op a (fun v => @under_lets _ (eC v) _ C)
-         | LetBinop _ _ op a b _ eC
-           => fun tC C => LetBinop op a b (fun v => @under_lets _ (eC v) _ C)
-         | LetTrinop _ _ _ op a b c _ eC
-           => fun tC C => LetTrinop op a b c (fun v => @under_lets _ (eC v) _ C)
-         | LetTrinop2Ret _ _ _ op a b c _ eC
-           => fun tC C => LetTrinop2Ret op a b c (fun v0 v1 => @under_lets _ (eC v0 v1) _ C)
-         | Abs _ _ f
-           => fun tC C => Abs (fun x => @under_lets _ (f x) tC C)
-         | Return _ a
-           => fun _ C => C a
-         end.
-
-    Fixpoint under_lets_no_abs {t} (e: expr var t) {struct e} :
-      forall {tC} (C:match t with
-                     | Arrow _ _ => expr var t
-                     | Tflat t => arg var t
-                     end -> expr var tC), expr var tC
-      := match e in (expr _ t) return forall {tC} (C:match t with
-                                                     | Arrow _ _ => expr var t
-                                                     | Tflat t => arg var t
-                                                     end -> expr var tC), expr var tC with
-         | LetUnop _ op a _ eC
-           => fun tC C => LetUnop op a (fun v => @under_lets_no_abs _ (eC v) _ C)
-         | LetBinop _ _ op a b _ eC
-           => fun tC C => LetBinop op a b (fun v => @under_lets_no_abs _ (eC v) _ C)
-         | LetTrinop _ _ _ op a b c _ eC
-           => fun tC C => LetTrinop op a b c (fun v => @under_lets_no_abs _ (eC v) _ C)
-         | LetTrinop2Ret _ _ _ op a b c _ eC
-           => fun tC C => LetTrinop2Ret op a b c (fun v0 v1 => @under_lets_no_abs _ (eC v0 v1) _ C)
-         | Abs _ _ f as e
-           => fun tC C => C e
-         | Return _ a
-           => fun _ C => C a
-         end.
-  End under_lets.
-
-  Fixpoint interp_under_arrows t1 {t} (e : @expr _ t) : interp_type (under_arrows t1 (fun _ => t))
-    := match t1 with
-       | Arrow s d => fun _ => @interp_under_arrows d t e
-       | _ => interp e
-       end.
-  Fixpoint interp_simple_arg {t} (e : @simple_arg _ t) : interp_type t
-    := match t return @simple_arg _ t -> interp_type t with
-       | Arrow s d => fun e _ => @interp_simple_arg d e
-       | Tflat t => fun e => interp_arg e
-       end e.
-  Fixpoint pointwise_eq_interp {t} : forall (f g : interp_type t), Prop
-    := match t return forall (f g : interp_type t), Prop with
-       | Arrow s d => fun f g => forall x, @pointwise_eq_interp d (f x) (g x)
-       | Tflat _ => fun f g => f = g
-       end.
-  Fixpoint eq_interp_under_arrows {t1 t} : forall (f g : interp_type (under_arrows t1 t)), Prop
-    := match t1 return forall (f g : interp_type (under_arrows t1 t)), Prop with
-       | Arrow s d => fun f g => forall x, @eq_interp_under_arrows d t (f x) (g x)
-       | Tflat _ => pointwise_eq_interp
-       end.
-  Module Export Instances.
-    Global Instance pointwise_eq_interp_Reflexive {t} : Reflexive (@pointwise_eq_interp t) | 1.
-    Proof. induction t; intro x; simpl in *; try reflexivity. Qed.
-    Global Instance eq_interp_under_arrows_Reflexive {t1 t} : Reflexive (@eq_interp_under_arrows t1 t) | 1.
-    Proof. induction t1; intro x; simpl in *; try reflexivity. Qed.
-    Global Instance pointwise_eq_interp_Transitive {t} : Transitive (@pointwise_eq_interp t) | 1.
-    Proof. induction t; intros ???; simpl in *; eauto using eq_trans, transitivity. Qed.
-    Global Instance eq_interp_under_arrows_Transitive {t1 t} : Transitive (@eq_interp_under_arrows t1 t) | 1.
-    Proof. induction t1; intros ???; simpl in *; etransitivity; eauto. Qed.
-    Global Instance pointwise_eq_interp_Symmetric {t} : Symmetric (@pointwise_eq_interp t) | 1.
-    Proof. induction t; intros ??; simpl in *; eauto using eq_sym, symmetry. Qed.
-    Global Instance eq_interp_under_arrows_Symmetric {t1 t} : Symmetric (@eq_interp_under_arrows t1 t) | 1.
-    Proof. induction t1; intros ??; simpl in *; symmetry; eauto. Qed.
-    Global Instance pointwise_eq_interp_Proper {t}
-      : Proper (@pointwise_eq_interp t ==> @pointwise_eq_interp t ==> Basics.flip Basics.impl)
-               (@Output.pointwise_eq_interp t).
-    Proof.
-      intros ?? H ?? H' H''.
-      repeat first [ assumption
-                   | symmetry; assumption
-                   | etransitivity; try eassumption; [] ].
-    Qed.
-  End Instances.
-
-  Lemma under_lets_correct {t} (e: @expr _ t) {tC}
-    (C: @simple_arg _ t -> @expr _ tC)
-    (C_Proper : forall a1 a2, interp_arg a1 = interp_arg a2 -> interp (C a1) = interp (C a2)) :
-    forall a, interp_simple_arg a = interp e -> eq_interp_under_arrows (interp (under_lets e C)) (interp_under_arrows t (C a)).
-  Proof.
-    induction e;
-      repeat (intuition (congruence || eauto) + simpl in * + rewrite_hyp !* + break_match
-              + match goal with H : _ |- _ => progress eauto using (fun x => f_equal (fun f => f x) H) end
-              + reflexivity
-              + (erewrite_hyp *; [ reflexivity | first [ eassumption | symmetry; eassumption ] ])).
-  Qed.
-
-  Local Notation expr_or_arg t := (match t with
-                                   | Arrow _ _ => @expr interp_type t
-                                   | Tflat t' => @arg interp_type t'
-                                   end).
-  Definition interp_expr_or_arg {t} (e : expr_or_arg t) : interp_type t
-    := match t return expr_or_arg t -> interp_type t with
-       | Arrow _ _ => interp
-       | Tflat _ => interp_arg
-       end e.
-
-  Lemma under_lets_no_abs_correct_pointwise {t} (e: @expr _ t) {tC}
-        (C: expr_or_arg t -> @expr _ tC)
-    (C_Proper : forall a1 a2, pointwise_eq_interp (interp_expr_or_arg a1) (interp_expr_or_arg a2) -> pointwise_eq_interp (interp (C a1)) (interp (C a2))) :
-    forall a, pointwise_eq_interp (interp_expr_or_arg a) (interp e) -> pointwise_eq_interp (interp (under_lets_no_abs e C)) (interp (C a)).
-  Proof.
-    induction e;
-      repeat (intuition (congruence || eauto || reflexivity) + ( simpl in * ) + break_match
-              + (rewrite_hyp *; []) + (rewrite_hyp *; [ reflexivity | ])
-              + match goal with H : _ |- _ => progress eauto using (fun x => f_equal (fun f => f x) H) end).
-  Qed.
-
-  Lemma under_lets_correct_pointwise {t} (e: @expr _ t) {tC}
-    (C: @simple_arg _ t -> @expr _ tC)
-    (C_Proper : forall a1 a2, pointwise_eq_interp (interp_arg a1) (interp_arg a2) -> pointwise_eq_interp (interp (C a1)) (interp (C a2))) :
-    forall a, pointwise_eq_interp (interp_simple_arg a) (interp e) -> eq_interp_under_arrows (interp (under_lets e C)) (interp_under_arrows t (C a)).
-  Proof.
-    induction e;
-      try solve [ repeat (intuition (congruence || eauto) + simpl in * + rewrite_hyp !* + break_match
-              + match goal with H : _ |- _ => progress eauto using (fun x => f_equal (fun f => f x) H) end) ].
-  Qed.
-
-  Section match_arg.
-    Context {var:vartype -> Type}.
-
-    Arguments arg _ _ : clear implicits.
-    Arguments simple_arg _ _ : clear implicits.
-    Arguments expr _ _ : clear implicits.
-
-    Definition match_arg_Prod' {t1} {t2} (a:arg var (Prod t1 t2)) : option (arg var t1 * arg var t2) :=
-      match a in arg _ t
-        return option (match t with | Prod _ _ => _ | _ => False end) with
-      | Pair _ a1 _ a2 => Some (a1, a2)
-      | _ => None
-      end.
-
-    Definition match_arg_Prod {t1} {t2} (a:arg var (Prod t1 t2)) : (arg var t1 * arg var t2).
-      refine match match_arg_Prod' a with
-      | Some (a1, a2) => (a1, a2)
-      | None => _ (* impossible *)
-      end.
-    Proof.
-      intros; constructor;
-        abstract (repeat match goal with
-        | [a: interp_type _ |- _] => destruct a; constructor; assumption
-        | [a: arg _ (Prod _ _) |- _] => inversion_clear a; try assumption
-        end).
-    Defined.
-
-    Global Arguments match_arg_Prod / : simpl nomatch.
-
-    Definition match_arg_Prod_Pair {t1 t2} (a1:arg var t1) (a2:arg var t2) :
-      match_arg_Prod (Pair a1 a2) = (a1, a2) := eq_refl.
-
-    Lemma match_arg_Prod_correct_helper {t} (a:arg var t) :
-      match t return arg var t -> Prop with
-      | Prod _ _ => fun a => forall a1 a2, match_arg_Prod a = (a1, a2) <-> a = Pair a1 a2
-      | _ => fun _ => True
-      end a.
-    Proof.
-      unfold match_arg_Prod; destruct a;
-        repeat match goal with
-        | _ => split
-        | _ => intro
-        | _ => progress simpl in *
-        | _ => break_match
-        | _ => intuition congruence
-        | H: _ |- _ => eapply (f_equal match_arg_Prod) in H
-        end.
-    Qed.
-
-    Lemma match_arg_Prod_correct {t1 t2} (a:arg _ (Prod t1 t2)) (a1:arg _ t1) (a2:arg _ t2) :
-      match_arg_Prod a = (a1, a2) <-> a = (Pair a1 a2).
-    Proof.
-      pose proof (match_arg_Prod_correct_helper a) as H; simpl in H; rewrite H; reflexivity.
-    Qed.
-
-    Lemma Pair_eq t0 t1 x0 x1 x0' x1' : @Pair var t0 x0 t1 x1 = @Pair var t0 x0' t1 x1' <-> (x0, x1) = (x0', x1').
-    Proof.
-      split; intro H; try congruence.
-      apply (f_equal match_arg_Prod) in H; assumption.
-    Qed.
-  End match_arg.
-
-  Fixpoint uninterp_arg {t} {struct t} : interp_flat_type t -> @arg interp_type t
-    := match t return interp_flat_type t -> @arg interp_type t with
-       | Prod t1 t2 => fun x => let (x1, x2) := x in
-                                Pair (@uninterp_arg t1 x1) (@uninterp_arg t2 x2)
-       | TW => @Var interp_type _
-       | Tbool => @Var interp_type _
-       | TZ => Const
-       end.
-
-  Lemma interp_arg_uninterp_arg : forall t (a:interp_flat_type t), interp_arg (uninterp_arg a) = a.
-  Proof.
-    induction t; simpl; intros; try reflexivity;
-      repeat break_match; subst; simpl; intuition try congruence.
-  Qed.
-
-  Lemma interp_simple_arg_uninterp_arg : forall (t : flat_type) (a:interp_type t), @interp_simple_arg t (@uninterp_arg t a) = a.
-  Proof.
-    apply interp_arg_uninterp_arg.
-  Qed.
-
-  Lemma interp_under_lets {t: flat_type} {tC: type}
-        (e: @expr _ t)
-        (C: @arg _ t -> @expr _ tC)
-        (C_Proper : forall a1 a2, interp_arg a1 = interp_arg a2 ->
-              interp (C a1) = interp (C a2)) :
-    pointwise_eq_interp (@interp tC (under_lets e C)) (@interp tC (C (@uninterp_arg t (interp e)))).
-  Proof.
-    intros; apply (@under_lets_correct t);
-    [ assumption
-    | rewrite interp_simple_arg_uninterp_arg; reflexivity ].
-  Qed.
-
-  Lemma interp_under_lets_flat {t: flat_type} {tC: flat_type}
-        (e: @expr _ t)
-        (C: @arg _ t -> @expr _ tC)
-        (C_Proper : forall a1 a2, interp_arg a1 = interp_arg a2 ->
-              interp (C a1) = interp (C a2)) :
-    @interp tC (under_lets e C)  = @interp tC (C (@uninterp_arg t (interp e))).
-  Proof.
-    apply (@interp_under_lets t tC); assumption.
-  Qed.
-
-  Lemma interp_under_lets_pointwise {t: flat_type} {tC: type}
-        (e: @expr _ t)
-        (C: @arg _ t -> @expr _ tC)
-        (C_Proper : forall a1 a2, pointwise_eq_interp (interp_arg a1) (interp_arg a2) ->
-              pointwise_eq_interp (interp (C a1)) (interp (C a2))) :
-    pointwise_eq_interp (@interp tC (under_lets e C)) (@interp tC (C (@uninterp_arg t (interp e)))).
-  Proof.
-    intros; apply (@under_lets_correct_pointwise t);
-    [ assumption
-    | rewrite interp_simple_arg_uninterp_arg; reflexivity ].
-  Qed.
-
-  Lemma interp_under_lets_no_abs_pointwise {t: flat_type} {tC: type}
-        (e: @expr _ t)
-        (C: expr_or_arg (Tflat t) -> @expr _ tC)
-        (C_Proper : forall a1 a2, pointwise_eq_interp (interp_expr_or_arg (t:=t) a1) (interp_expr_or_arg (t:=t) a2) ->
-              pointwise_eq_interp (interp (C a1)) (interp (C a2))) :
-    pointwise_eq_interp (@interp tC (under_lets_no_abs e C)) (@interp tC (C (@uninterp_arg t (interp e)))).
-  Proof.
-    intros; apply (@under_lets_no_abs_correct_pointwise t); simpl;
-    [ assumption
-    | rewrite interp_arg_uninterp_arg; reflexivity ].
-  Qed.
-
-  Section wf.
-    Context {var1 var2 : vartype -> Type}.
-
-    Local Notation "x ≡ y" := (existT _ _ (x, y)).
-
-    Inductive wf_arg : list (sigT (fun t => var1 t * var2 t))%type -> forall {t}, @arg var1 t -> @arg var2 t -> Prop :=
-    | WfConst : forall G t n, wf_arg G (Const (t := t) n) (Const n)
-    | WfSpZConst : forall G n, wf_arg G (SpZConst n) (SpZConst n)
-    | WfVar : forall G (t : vartype) x x', In (x ≡ x') G -> @wf_arg G t (Var x) (Var x')
-    | WfPair : forall G {t1} {t2} (e1: @arg var1 t1) (e2: @arg var1 t2)
-                      (e1': @arg var2 t1) (e2': @arg var2 t2),
-        wf_arg G e1 e1'
-        -> wf_arg G e2 e2'
-        -> wf_arg G (Pair e1 e2) (Pair e1' e2').
-
-    Inductive wf : list (sigT (fun t => var1 t * var2 t))%type -> forall {t}, @expr var1 t -> @expr var2 t -> Prop :=
-    | WfLetUnop : forall G {t1} (op : nop 1 1 t1 _) (e1:@arg var1 t1) (e1':@arg var2 t1)
-                         tC b b',
-        wf_arg G e1 e1'
-        -> (forall x1 x2, wf ((x1 ≡ x2) :: G) (b x1) (b' x2))
-        -> wf G (LetUnop (tC := tC) op e1 b) (LetUnop (tC := tC) op e1' b')
-    | WfLetBinop : forall G {t10 t11} (op : nop 2 1 (t10, t11) _)
-                       (e10:@arg var1 t10) (e11:@arg var1 t11)
-                       (e10':@arg var2 t10) (e11':@arg var2 t11)
-                       tC b b',
-        wf_arg G e10 e10'
-        -> wf_arg G e11 e11'
-        -> (forall x1 x2, wf ((x1 ≡ x2) :: G) (b x1) (b' x2))
-        -> wf G (LetBinop (tC := tC) op e10 e11 b) (LetBinop (tC := tC) op e10' e11' b')
-    | WfLetTrinop : forall G {t10 t11 t12} (op : nop 3 1 (t10, t11, t12) _)
-                       (e10:@arg var1 t10) (e11:@arg var1 t11) (e12:@arg var1 t12)
-                       (e10':@arg var2 t10) (e11':@arg var2 t11) (e12':@arg var2 t12)
-                       tC b b',
-        wf_arg G e10 e10'
-        -> wf_arg G e11 e11'
-        -> wf_arg G e12 e12'
-        -> (forall x1 x2, wf ((x1 ≡ x2) :: G) (b x1) (b' x2))
-        -> wf G (LetTrinop (tC := tC) op e10 e11 e12 b) (LetTrinop (tC := tC) op e10' e11' e12' b')
-    | WfLetTrinop2Ret : forall G {t10 t11 t12} (op : nop 3 2 (t10, t11, t12) _)
-                       (e10:@arg var1 t10) (e11:@arg var1 t11) (e12:@arg var1 t12)
-                       (e10':@arg var2 t10) (e11':@arg var2 t11) (e12':@arg var2 t12)
-                       tC b b',
-        wf_arg G e10 e10'
-        -> wf_arg G e11 e11'
-        -> wf_arg G e12 e12'
-        -> (forall x10 x11 x20 x21, wf ((x11 ≡ x21) :: (x10 ≡ x20) :: G) (b x10 x11) (b' x20 x21))
-        -> wf G (LetTrinop2Ret (tC := tC) op e10 e11 e12 b) (LetTrinop2Ret (tC := tC) op e10' e11' e12' b')
-    | WfAbs : forall G t1 t2 e e',
-        (forall x1 x2, wf ((x1 ≡ x2) :: G) (e x1) (e' x2))
-        -> wf G (@Abs _ t1 t2 e) (Abs e')
-    | WfReturn : forall G t x x', wf_arg G x x' -> wf G (Return (t := t) x) (Return x').
-
-  End wf.
-
-  Definition Wf {t} (E : @Expr t) := forall var1 var2, wf nil (E var1) (E var2).
-
-End Output.
-
-Section compile.
-  Context {ivar : vartype -> Type}.
-  Context {ovar : vartype -> Type}.
-
-  Fixpoint reify_interped {t} : interp_flat_type t -> @Output.expr ovar t
-    := match t return interp_type t -> @Output.expr ovar t with
-       | Prod t0 t1
-         => fun x0x1
-            => @Output.under_lets
-                 _ _ (@reify_interped t0 (fst x0x1)) _
-                 (fun x0
-                  => @Output.under_lets
-                       _ _ (@reify_interped t1 (snd x0x1)) _
-                       (fun x1
-                        => Output.Return (Output.Pair x0 x1)))
-       | TZ => fun n => Output.Return (Output.Const n)
-       | TW => fun n => Output.Return (Output.Const n)
-       | Tbool => fun n => Output.Return (Output.Const n)
-       end.
-
-  Fixpoint compile {t} (e:@Input.expr (@Output.arg ovar) t) : @Output.expr ovar t
-    := match e in @Input.expr _ t return @Output.expr ovar t with
-           | Input.Const _ n => reify_interped n
-           | Input.SpZConst n => Output.Return (Output.SpZConst n)
-           | Input.Var _ n => Output.Return n
-           | Input.Unop _ TW op a =>
-             Output.under_lets (@compile _ a) (fun arg1 =>
-                Output.LetUnop op arg1 (fun v => Output.Return (Output.Var v)))
-           | Input.Unop _ _ op a => match op with OPldi => fun x => x end (* whee small inversion magic *)
-           | Input.Binop _ _ TW op a b =>
-             Output.under_lets (@compile _ a) (fun arg1 =>
-             Output.under_lets (@compile _ b) (fun arg2 =>
-                Output.LetBinop op arg1 arg2 (fun v => Output.Return (Output.Var v))))
-           | Input.Binop _ _ _ op a b => match op with OPldi => fun x => x end (* whee small inversion magic *)
-           | Input.Trinop _ _ _ TW op a b c =>
-             Output.under_lets (@compile _ a) (fun arg1 =>
-             Output.under_lets (@compile _ b) (fun arg2 =>
-             Output.under_lets (@compile _ c) (fun arg3 =>
-                Output.LetTrinop op arg1 arg2 arg3 (fun v => Output.Return (Output.Var v)))))
-           | Input.Trinop _ _ _ _ op a b c => match op with OPldi => fun x => x end (* whee small inversion magic *)
-           | Input.Trinop2Ret _ _ _ (Tbool, TW) op a b c =>
-             Output.under_lets (@compile _ a) (fun arg1 =>
-             Output.under_lets (@compile _ b) (fun arg2 =>
-             Output.under_lets (@compile _ c) (fun arg3 =>
-                Output.LetTrinop2Ret op arg1 arg2 arg3 (fun v0 v1 => Output.Return (Output.Pair (Output.Var v0) (Output.Var v1))))))
-           | Input.Trinop2Ret _ _ _ _ op a b c => match op with OPldi => fun x => x end (* whee small inversion magic *)
-    | Input.Let _ ex _ eC =>
-       Output.under_lets (@compile _ ex) (fun arg => @compile _ (eC arg))
-    | Input.Pair _ e1 _ e2 =>
-       Output.under_lets (@compile _ e1) (fun arg1 =>
-          Output.under_lets (@compile _ e2) (fun arg2 =>
-             Output.Return (Output.Pair arg1 arg2)))
-    | Input.MatchPair _ _ ep _ eC =>
-        Output.under_lets (@compile _ ep) (fun arg =>
-          let (a1, a2) := Output.match_arg_Prod arg in @compile _ (eC a1 a2))
-    | Input.Abs _ _ f => Output.Abs (fun x => @compile _ (f (Output.Var x)))
-           end.
-  End compile.
-
-Definition Compile {t} (e:Input.Expr t) : Output.Expr t := fun var =>
-  compile (e (@Output.arg var)).
-
-Lemma interp_reify_interped t n
-  : Output.interp (t := Tflat t) (reify_interped n) = n.
-Proof.
-  induction t; simpl.
-  { repeat break_match; reflexivity. }
-  { repeat first [ reflexivity
-                 | rewrite !Output.interp_under_lets
-                 | rewrite !Output.interp_arg_uninterp_arg
-                 | rewrite <- surjective_pairing
-                 | intro
-                 | progress simpl in *
-                 | rewrite_hyp !* ]. }
-Qed.
-
-Lemma compile_correct {t} e1 e2 G (wf:Input.wf G e1 e2) :
-  List.Forall (fun v => let 'existT _ (x, a) := v in Output.interp_arg a = x) G ->
-    Output.pointwise_eq_interp (t := t) (Output.interp (compile e2)) (Input.interp e1).
-Proof.
-  induction wf;
-    repeat repeat match goal with
-           | [ |- ?R ?x ?x ] => reflexivity
-    | [HIn:In ?x ?l, HForall:Forall _ ?l |- _ ] =>
-      (pose proof (proj1 (Forall_forall _ _) HForall _ HIn); clear HIn)
-    | [ H : Output.match_arg_Prod _ = (_, _) |- _ ] =>
-      apply Output.match_arg_Prod_correct in H
-    | [ H : Output.Pair _ _ = Output.Pair _ _ |- _ ] =>
-      apply Output.Pair_eq in H
-    | [ H : (_, _) = (_, _) |- _ ] => inversion H; clear H
-    | _ => progress intros
-    | _ => progress simpl in *
-    | _ => progress subst
-    | _ => progress specialize_by assumption
-    | _ => progress break_match
-    | _ => rewrite !Output.interp_under_lets_pointwise
-    | _ => rewrite !Output.interp_under_lets_flat
-    | _ => rewrite !Output.interp_under_lets
-    | _ => rewrite !interp_reify_interped
-    | _ => rewrite !Output.interp_arg_uninterp_arg
-    | _ => rewrite <- !surjective_pairing
-    | _ => progress erewrite_hyp !*
-    | _ => apply Forall_cons
-    | [ |- context[match ?op with OPldi => _ | _ => _ end] ]
-      => solve [ exfalso; refine (match op with OPldi => idProp end) ]
-    | _ => solve [intuition (congruence || eauto)]
-    | [ H : _ |- Output.pointwise_eq_interp _ _ ] => apply H
-    end.
-Qed.
-
-Lemma Compile_correct {t} (E:Input.Expr t) (WfE:Input.Wf E) :
-  Output.pointwise_eq_interp (Output.Interp (Compile E)) (Input.Interp E).
-Proof. eapply compile_correct; eauto. Qed.
-
-Section symbolic.
+Section expression.
+  Context (ops : fancy_machine.instructions (2 * 128)) (props : fancy_machine.arithmetic ops) (modulus : Z) (m' : Z) (Hm : modulus <> 0) (H : 0 <= modulus < 2^256) (Hm' : 0 <= m' < 2^256).
+  Let H' : 0 <= 256 <= 256. omega. Qed.
+  Let H'' : 0 < 256. omega. Qed.
+  Let props' := ZLikeProperties_of_ArchitectureBoundedOps ops modulus H 256 H' H''.
+  Let ops' := (ZLikeOps_of_ArchitectureBoundedOps ops modulus 256).
+  Local Notation fst' := (@fst fancy_machine.W fancy_machine.W).
+  Local Notation snd' := (@snd fancy_machine.W fancy_machine.W).
+  Definition ldi' : load_immediate
+                     (@ZBounded.SmallT (2 ^ 256) (2 ^ 256) modulus
+                                       (@ZLikeOps_of_ArchitectureBoundedOps 128 ops modulus 256)) := _.
+  Let isldi : is_load_immediate ldi' := _.
+  Definition pre_f := (fun v => (reduce_via_partial (2^256) modulus (props := props') (ldi' m') I Hm (fst' v, snd' v))).
+  Definition f := (fun v => proj1_sig (pre_f v)).
+
+  Local Arguments proj1_sig _ _ !_ / .
+  Local Arguments ZBounded.CarryAdd / .
+  Local Arguments ZBounded.ConditionalSubtract / .
+  Local Arguments ZBounded.ConditionalSubtractModulus / .
+  Local Arguments ZLikeOps_of_ArchitectureBoundedOps / .
+  Local Arguments ZBounded.DivBy_SmallBound / .
+  Local Arguments f / .
+  Local Arguments pre_f / .
+  Local Arguments ldi' / .
+  Local Arguments reduce_via_partial / .
+
+  Definition expression'
+    := Eval simpl in f.
+  Definition expression
+    := Eval cbv beta delta [expression' fst snd] in
+        fun v => let RegMod := fancy_machine.ldi modulus in
+                 let RegPInv := fancy_machine.ldi m' in
+                 let RegZero := fancy_machine.ldi 0 in
+                 expression' v.
+  Definition expression_eq v : fancy_machine.decode (expression v) = _
+    := proj1 (proj2_sig (pre_f v) I).
+  Definition expression_correct
+             R' HR0 HR1
+             v
+             Hv
+    : ZUtil.Z.equiv_modulo _ (fancy_machine.decode (expression v)) _
+      /\ 0 <= fancy_machine.decode (expression v) < _
+    := @ZBounded.reduce_via_partial_correct (2^256) modulus _ props' (ldi' m') I Hm R' HR0 HR1 v I Hv.
+End expression.
+
+Section reflection.
+  Context (ops : fancy_machine.instructions (2 * 128)).
   Local Set Boolean Equality Schemes.
   Local Set Decidable Equality Schemes.
-  (** Holds decidably-equal versions of raw expressions, for lookup. *)
-  Inductive sop : Set :=
-    SOPldi | SOPshrd | SOPshl | SOPshr | SOPmkl | SOPadc | SOPsubc | SOPmulhwll | SOPmulhwhl | SOPmulhwhh | SOPselc | SOPaddm.
-  Inductive SymbolicExpr : Set :=
-  | SConstZ : Z -> SymbolicExpr
-  | SSpZConst : SpecialZConst -> SymbolicExpr
-  | SConstBool : bool -> SymbolicExpr
-  | SConstW : nat -> SymbolicExpr
-  | SVar : vartype -> nat -> SymbolicExpr
-  | SPair : SymbolicExpr -> SymbolicExpr -> SymbolicExpr
-  | SUnOp : sop -> SymbolicExpr -> SymbolicExpr
-  | SBinOp : sop -> SymbolicExpr -> SymbolicExpr -> SymbolicExpr
-  | STrinOp : sop -> SymbolicExpr -> SymbolicExpr -> SymbolicExpr -> SymbolicExpr
-  | STrinOp2Ret : sop -> SymbolicExpr -> SymbolicExpr -> SymbolicExpr -> SymbolicExpr.
-End symbolic.
+  Inductive base_type := TZ | Tbool | TW.
+  Definition interp_base_type (v : base_type) : Type :=
+    match v with
+    | TZ => Z
+    | Tbool => bool
+    | TW => fancy_machine.W
+    end.
+  Local Notation tZ := (Tbase TZ).
+  Local Notation tbool := (Tbase Tbool).
+  Local Notation tW := (Tbase TW).
+  Local Open Scope ctype_scope.
+  Inductive op : flat_type base_type -> flat_type base_type -> Type :=
+  | OPldi     : op tZ tW
+  | OPshrd    : op (tW * tW * tZ) tW
+  | OPshl     : op (tW * tZ) tW
+  | OPshr     : op (tW * tZ) tW
+  | OPmkl     : op (tW * tZ) tW
+  | OPadc     : op (tW * tW * tbool) (tbool * tW)
+  | OPsubc    : op (tW * tW * tbool) (tbool * tW)
+  | OPmulhwll : op (tW * tW) tW
+  | OPmulhwhl : op (tW * tW) tW
+  | OPmulhwhh : op (tW * tW) tW
+  | OPselc    : op (tbool * tW * tW) tW
+  | OPaddm    : op (tW * tW * tW) tW.
 
-Section CSE.
-  Context {var : vartype -> Type}.
-  Let svar t := (var t * SymbolicExpr)%type.
-  Let mapping := (list (svar TW) * list (svar Tbool))%type.
-
-  Fixpoint lookup' {t} (sv : SymbolicExpr) (xs : list (svar t)) {struct xs} : option (var t) :=
-    match xs with
-    | nil => None
-    | (x, sv') :: xs' =>
-      if SymbolicExpr_beq sv' sv
-      then Some x
-      else lookup' sv xs'
-    end.
-  Definition lookup t (sv : SymbolicExpr) (xs : mapping) : option (var t) :=
-    match t with
-    | TW => lookup' sv (fst xs)
-    | Tbool => lookup' sv (snd xs)
-    end.
-  Definition mapping_nth_error (xs : mapping) t n : option (svar t) :=
-    match t with
-    | TW => nth_error (fst xs) n
-    | Tbool => nth_error (snd xs) n
-    end.
-  Definition symbolicify_var {t : vartype} (v : var t) (xs : mapping) : SymbolicExpr :=
-    SVar t (match t with
-            | TW => length (fst xs)
-            | Tbool => length (snd xs)
-            end).
-  Definition add_mapping {t} (v : var t) (sv : SymbolicExpr) (xs : mapping) : mapping :=
-    match t return var t -> mapping with
-    | TW => fun v => ((v, sv) :: fst xs, snd xs)
-    | Tbool => fun v => (fst xs, (v, sv) :: snd xs)
-    end v.
-  Definition sop_eval_dep (op : sop)
-    := match op return match op with SOPldi => _ | _ => _ end with
-       | SOPldi => OPldi
-       | SOPshrd => OPshrd
-       | SOPshl => OPshl
-       | SOPshr => OPshr
-       | SOPmkl => OPmkl
-       | SOPadc => OPadc
-       | SOPsubc => OPsubc
-       | SOPmulhwll => OPmulhwll
-       | SOPmulhwhl => OPmulhwhl
-       | SOPmulhwhh => OPmulhwhh
-       | SOPselc => OPselc
-       | SOPaddm => OPaddm
-       end.
-  Definition sop_eval nret (op : sop) (t : tuple flat_type nret) : option (sigT (fun nargs : nat => sigT (fun args : tuple flat_type nargs => nop nargs nret args t)))
-    := match nret return forall t : tuple flat_type nret, option (sigT (fun nargs : nat => sigT (fun args : tuple flat_type nargs => nop nargs nret args t))) with
-       | 1%nat => fun t => match op, t with
-                     | SOPldi as op, TW
-                     | SOPshrd as op, TW
-                     | SOPshr as op, TW
-                     | SOPshl as op, TW
-                     | SOPmkl as op, TW
-                     | SOPmulhwll as op, TW
-                     | SOPmulhwhl as op, TW
-                     | SOPmulhwhh as op, TW
-                     | SOPselc as op, TW
-                     | SOPaddm as op, TW
-                       => Some (existT _ _ (existT _ _ (sop_eval_dep op)))
-                     | _, _ => None
-                     end
-       | 2%nat => fun t => match op, t with
-                     | SOPadc as op, (Tbool, TW)
-                     | SOPsubc as op, (Tbool, TW)
-                       => Some (existT _ _ (existT _ _ (sop_eval_dep op)))
-                     | _, _ => None
-                     end
-       | _ => fun _ => None
-       end t.
-  Fixpoint symbolic_preeval {t} (xs : mapping) (e : SymbolicExpr) : option (@Output.expr var t)
-    := match e, t return option (@Output.expr var t) with
-           | SConstZ v, TZ as t
-           | SConstBool v, Tbool as t
-             => Some (Output.Return (Output.Const (t := t) v))
-           | SConstZ _, _ => None
-           | SConstBool _, _ => None
-           | SSpZConst v, TZ => Some (Output.Return (Output.SpZConst v))
-           | SSpZConst _, _ => None
-           | SConstW n, TW as t => option_map (fun x => Output.Return (Output.Var (fst x)))
-                                             (mapping_nth_error xs t n)
-           | SConstW _, _ => None
-           | SVar Tbool n, Tbool as t
-           | SVar TW n, TW as t
-             => option_map (fun x => Output.Return (Output.Var (fst x)))
-                          (mapping_nth_error xs t n)
-           | SVar _ _, _ => None
-           | SPair x y, Prod tx ty
-             => match @symbolic_preeval tx xs x, @symbolic_preeval ty xs y with
-               | Some x', Some y' => Some (Output.under_lets x' (fun x0 => Output.under_lets y' (fun y0 => Output.Return (Output.Pair x0 y0))))
-               | _, _ => None
-               end
-           | SPair _ _, _ => None
-           | SUnOp op x0, TW as t
-             => match sop_eval 1 op t with
-               | Some (existT 1%nat (existT x0t opv))
-                 => option_map
-                     (fun x0' : Output.expr x0t
-                      => Output.under_lets
-                           x0' (fun x0' => Output.LetUnop
-                                             opv x0'
-                                             (fun v => Output.Return (Output.Var v))))
-                     (@symbolic_preeval x0t xs x0)
-               | _ => None
-               end
-           | SUnOp _ _, _ => None
-           | SBinOp op x0 x1, TW as t
-             => match sop_eval 1 op t with
-               | Some (existT 2%nat (existT (x0t, x1t) opv))
-                 => match @symbolic_preeval x0t xs x0, @symbolic_preeval x1t xs x1 with
-                   | Some x0', Some x1'
-                     => Some
-                         (Output.under_lets
-                            x0' (fun x0' =>
-                                   Output.under_lets
-                                     x1' (fun x1' =>
-                                            Output.LetBinop
-                                              opv x0' x1'
-                                              (fun v => Output.Return (Output.Var v)))))
-                   | _, _ => None
-                   end
-               | _ => None
-               end
-           | SBinOp _ _ _, _ => None
-           | STrinOp op x0 x1 x2, TW as t
-             => match sop_eval 1 op t with
-               | Some (existT 3%nat (existT (x0t, x1t, x2t) opv))
-                 => match @symbolic_preeval x0t xs x0, @symbolic_preeval x1t xs x1, @symbolic_preeval x2t xs x2 with
-                   | Some x0', Some x1', Some x2'
-                     => Some
-                         (Output.under_lets
-                            x0' (fun x0' =>
-                                   Output.under_lets
-                                     x1' (fun x1' =>
-                                            Output.under_lets
-                                              x2' (fun x2' => Output.LetTrinop
-                                                             opv x0' x1' x2'
-                                                             (fun v => Output.Return (Output.Var v))))))
-                   | _, _, _ => None
-                   end
-               | _ => None
-               end
-           | STrinOp _ _ _ _, _ => None
-           | STrinOp2Ret op x0 x1 x2, (Prod Tbool TW) as t
-             => match sop_eval 2 op (Tbool:flat_type, TW:flat_type) with
-               | Some (existT 3%nat (existT (x0t, x1t, x2t) opv))
-                 => match @symbolic_preeval x0t xs x0, @symbolic_preeval x1t xs x1, @symbolic_preeval x2t xs x2 with
-                   | Some x0', Some x1', Some x2'
-                     => Some
-                         (Output.under_lets
-                            x0' (fun x0' =>
-                                   Output.under_lets
-                                     x1' (fun x1' =>
-                                            Output.under_lets
-                                              x2' (fun x2' => Output.LetTrinop2Ret
-                                                             opv x0' x1' x2'
-                                                             (fun c v => Output.Return (Output.Pair (Output.Var c) (Output.Var v)))))))
-                   | _, _, _ => None
-                   end
-               | _ => None
-               end
-           | STrinOp2Ret _ _ _ _, _ => None
+  Definition interp_op src dst (f : op src dst)
+    : interp_flat_type_gen interp_base_type src -> interp_flat_type_gen interp_base_type dst
+    := match f in op s d return interp_flat_type_gen _ s -> interp_flat_type_gen _ d with
+       | OPldi     => ldi
+       | OPshrd    => fun xyz => let '(x, y, z) := eta3 xyz in shrd x y z
+       | OPshl     => fun xy => let '(x, y) := eta xy in shl x y
+       | OPshr     => fun xy => let '(x, y) := eta xy in shr x y
+       | OPmkl     => fun xy => let '(x, y) := eta xy in mkl x y
+       | OPadc     => fun xyz => let '(x, y, z) := eta3 xyz in adc x y z
+       | OPsubc    => fun xyz => let '(x, y, z) := eta3 xyz in subc x y z
+       | OPmulhwll => fun xy => let '(x, y) := eta xy in mulhwll x y
+       | OPmulhwhl => fun xy => let '(x, y) := eta xy in mulhwhl x y
+       | OPmulhwhh => fun xy => let '(x, y) := eta xy in mulhwhh x y
+       | OPselc    => fun xyz => let '(x, y, z) := eta3 xyz in selc x y z
+       | OPaddm    => fun xyz => let '(x, y, z) := eta3 xyz in addm x y z
        end.
 
-  Fixpoint cseArg {t} (v : @Output.arg svar t) (xs : mapping) {struct v}
-    : @Output.arg var t * option SymbolicExpr
-    := match v in Output.arg t return Output.arg t * option SymbolicExpr with
-       | Output.Const Tbool v'
-         => let sv := SConstBool v' in
-           (match lookup Tbool sv xs with
-            | Some val => Output.Var val
-            | None => Output.Const v'
-            end,
-            Some sv)
-       | Output.Const TZ v'
-         => (Output.Const v', Some (SConstZ v'))
-       | Output.SpZConst v'
-         => (Output.SpZConst v', Some (SSpZConst v'))
-       | Output.Const _ v' => (Output.Const v', None)
-       | Output.Var t v'
-         => (Output.Var (match lookup t (snd v') xs with
-                        | Some val => val
-                        | None => fst v'
-                        end),
-            Some (snd v'))
-       | Output.Pair _ v0 _ v1
-         => let '(v0v, v0s) := eta (@cseArg _ v0 xs) in
-           let '(v1v, v1s) := eta (@cseArg _ v1 xs) in
-           (Output.Pair v0v v1v,
-            match v0s, v1s with
-            | Some v0', Some v1' => Some (SPair v0' v1')
-            | _, _ => None
-            end)
+  Inductive SConstT := ZConst (_ : Z) | BoolConst (_ : bool) | INVALID_CONST.
+  Inductive op_code : Set :=
+  | SOPldi | SOPshrd | SOPshl | SOPshr | SOPmkl | SOPadc | SOPsubc
+  | SOPmulhwll | SOPmulhwhl | SOPmulhwhh | SOPselc | SOPaddm.
+
+  Definition symbolicify_const (t : base_type) : interp_base_type t -> SConstT
+    := match t with
+       | TZ => fun x => ZConst x
+       | Tbool => fun x => BoolConst x
+       | TW => fun x => INVALID_CONST
        end.
-  Definition cseOp {narg nret t1 t2} (op : @nop narg nret t1 t2) : sop
-    := match op with
+  Definition symbolicify_op s d (v : op s d) : op_code
+    := match v with
        | OPldi => SOPldi
        | OPshrd => SOPshrd
        | OPshl => SOPshl
@@ -1150,529 +134,50 @@ Section CSE.
        | OPaddm => SOPaddm
        end.
 
-  Definition cseExprHelper1
-             (cseExpr : forall t (v : @Output.expr svar t) (xs : mapping), @Output.expr var t)
-             (xs : mapping)
-             {tC}
-             (f : svar TW -> @Output.expr svar tC)
-             (sv : option SymbolicExpr)
-             (default_head : (var TW -> @Output.expr var tC) -> @Output.expr var tC)
-    : @Output.expr var tC
-    := match option_map (fun sv' => (sv', lookup _ sv' xs)) sv with
-       | Some (sv', Some v') => @cseExpr _ (f (v', sv')) xs
-       | Some (sv', None)    => default_head (fun v => @cseExpr _ (f (v, sv')) (add_mapping v sv' xs))
-       | None                => default_head (fun v => let sv' := symbolicify_var v xs in
-                                                       @cseExpr _ (f (v, sv')) (add_mapping v sv' xs))
-       end.
-  Definition cseExprHelper2
-             (cseExpr : forall t (v : @Output.expr svar t) (xs : mapping), @Output.expr var t)
-             (xs : mapping)
-             {tC}
-             (f : svar Tbool -> svar TW -> @Output.expr svar tC)
-             (sv : option SymbolicExpr)
-             (default_head : (var Tbool -> var TW -> @Output.expr var tC) -> @Output.expr var tC)
-    : @Output.expr var tC
-    := match option_map (fun sv' => (sv', lookup Tbool sv' xs, lookup TW sv' xs)) sv with
-       | Some (sv', Some vb', Some vw')
-         => @cseExpr _ (f (vb', sv') (vw', sv')) xs
-       | Some (sv', _, _)
-         => default_head (fun vb vw => @cseExpr _ (f (vb, sv') (vw, sv'))
-                                                (add_mapping vw sv' (add_mapping vb sv' xs)))
-       | None
-         => default_head (fun vb vw => let svb' := symbolicify_var vb xs in
-                                       let svw' := symbolicify_var vw xs in
-                                       @cseExpr _ (f (vb, svb') (vw, svw'))
-                                                (add_mapping vw svw' (add_mapping vb svb' xs)))
-       end.
-  Definition cseExpr_step
-             (cseExpr : forall {t} (v : @Output.expr svar t) (xs : mapping), @Output.expr var t)
-             {t} (v : @Output.expr svar t) (xs : mapping)
-    : @Output.expr var t
-    := match v in Output.expr t return Output.expr t with
-       | Output.LetUnop _ op x0 _ f
-         => let sop := cseOp op in
-            let '(x0v, x0s) := eta (cseArg x0 xs) in
-            let sv := match x0s with
-                      | Some x0' => Some (SUnOp sop x0')
-                      | _ => None
-                      end in
-            let default_head := Output.LetUnop op x0v in
-            cseExprHelper1 (@cseExpr) xs f sv default_head
-       | Output.LetBinop _ _ op x0 x1 _ f
-         => let sop := cseOp op in
-            let '(x0v, x0s) := eta (cseArg x0 xs) in
-            let '(x1v, x1s) := eta (cseArg x1 xs) in
-            let sv := match x0s, x1s with
-                      | Some x0', Some x1' => Some (SBinOp sop x0' x1')
-                      | _, _ => None
-                      end in
-            let default_head := Output.LetBinop op x0v x1v in
-            cseExprHelper1 (@cseExpr) xs f sv default_head
-       | Output.LetTrinop _ _ _ op x0 x1 x2 _ f
-         => let sop := cseOp op in
-            let '(x0v, x0s) := eta (cseArg x0 xs) in
-            let '(x1v, x1s) := eta (cseArg x1 xs) in
-            let '(x2v, x2s) := eta (cseArg x2 xs) in
-            let sv := match x0s, x1s, x2s with
-                      | Some x0', Some x1', Some x2' => Some (STrinOp sop x0' x1' x2')
-                      | _, _, _ => None
-                      end in
-            let default_head := Output.LetTrinop op x0v x1v x2v in
-            cseExprHelper1 (@cseExpr) xs f sv default_head
-       | Output.LetTrinop2Ret _ _ _ op x0 x1 x2 _ f
-         => let sop := cseOp op in
-            let '(x0v, x0s) := eta (cseArg x0 xs) in
-            let '(x1v, x1s) := eta (cseArg x1 xs) in
-            let '(x2v, x2s) := eta (cseArg x2 xs) in
-            let sv := match x0s, x1s, x2s with
-                      | Some x0', Some x1', Some x2' => Some (STrinOp2Ret sop x0' x1' x2')
-                      | _, _, _ => None
-                      end in
-            let default_head := Output.LetTrinop2Ret op x0v x1v x2v in
-            cseExprHelper2 (@cseExpr) xs f sv default_head
-       | Output.Return _ x => Output.Return (fst (cseArg x xs))
-       | Output.Abs _ _ f => Output.Abs (fun x => let sx := symbolicify_var x xs in
-                                                  @cseExpr _ (f (x, sx)) (add_mapping x sx xs))
-       end.
-End CSE.
-Definition symbolic_eval {t} xs sv := option_map Output.interp (@symbolic_preeval _ t xs sv).
-Fixpoint cseExpr' {var t} v xs := @cseExpr_step var (@cseExpr' var) t v xs.
+  Definition CSE {t} e := @CSE base_type SConstT op_code base_type_beq SConstT_beq op_code_beq internal_base_type_dec_bl interp_base_type op symbolicify_const symbolicify_op t e (fun _ => nil).
+End reflection.
+Section instances.
+  Context {ops : fancy_machine.instructions (2 * 128)}.
+  Global Instance: forall x, reify_op op (ldi x) 1 OPldi := fun _ => I.
+  Global Instance: forall x y z, reify_op op (shrd x y z) 3 OPshrd := fun _ _ _ => I.
+  Global Instance: forall x y, reify_op op (shl x y) 2 OPshl := fun _ _ => I.
+  Global Instance: forall x y, reify_op op (shr x y) 2 OPshr := fun _ _ => I.
+  Global Instance: forall x y, reify_op op (mkl x y) 2 OPmkl := fun _ _ => I.
+  Global Instance: forall x y z, reify_op op (adc x y z) 3 OPadc := fun _ _ _ => I.
+  Global Instance: forall x y z, reify_op op (subc x y z) 3 OPsubc := fun _ _ _ => I.
+  Global Instance: forall x y, reify_op op (mulhwll x y) 2 OPmulhwll := fun _ _ => I.
+  Global Instance: forall x y, reify_op op (mulhwhl x y) 2 OPmulhwhl := fun _ _ => I.
+  Global Instance: forall x y, reify_op op (mulhwhh x y) 2 OPmulhwhh := fun _ _ => I.
+  Global Instance: forall x y z, reify_op op (selc x y z) 3 OPselc := fun _ _ _ => I.
+  Global Instance: forall x y z, reify_op op (addm x y z) 3 OPaddm := fun _ _ _ => I.
+  Global Instance: reify type Z := TZ.
+  Global Instance: reify type bool := Tbool.
+  Global Instance: reify type fancy_machine.W := TW.
+End instances.
+Ltac Reify' e := Reify.Reify' base_type (interp_base_type _) op e.
+Ltac Reify e := Reify.Reify base_type (interp_base_type _) op e.
+Ltac Reify_rhs := Reify.Reify_rhs base_type (interp_base_type _) op (interp_op _).
 
-Fixpoint cseExpr {var}
-         {t} (v : @Output.expr _ t) xs
-  := match v in Output.expr t return @Output.expr var t with
-     | Output.Abs _ _ f => Output.Abs (fun x => let sx := symbolicify_var x xs in
-                                                @cseExpr _ _ (f (x, sx)) (add_mapping x sx xs))
-     | v => @cseExpr'
-              var _
-              (Output.LetUnop OPldi (Output.Const (0:interp_type TZ)) (fun RegZero =>
-               Output.LetUnop OPldi (Output.SpZConst Cmodulus) (fun RegMod =>
-               Output.LetUnop OPldi (Output.SpZConst Cm') (fun RegPInv =>
-               v))))
-              xs
-     end.
+Section reflected.
+  Context (ops : fancy_machine.instructions (2 * 128)).
+  Definition rexpression : Syntax.Expr base_type (interp_base_type _) op (Arrow TZ (Arrow TZ (Arrow TW (Arrow TW (Tbase TW))))).
+  Proof.
+    let v := (eval cbv beta delta [expression] in (fun modulus m' x y => expression ops modulus m' (x, y))) in
+    let v := Reify v in
+    exact v.
+  Defined.
 
-Definition CSE {t} (e:Output.Expr t) : Output.Expr t := fun var =>
-  @cseExpr var t (e _) (nil, nil).
-
-Local Ltac specialize_vartype :=
-  repeat match goal with
-         | [ H : forall x : vartype, _ |- _ ]
-           => pose proof (H Tbool); pose proof (H TW); clear H
-         end.
-
-Lemma lookup_correct
-      (var := interp_type)
-      (svar := fun t => (var t * SymbolicExpr)%type)
-      (mapping := (list (svar TW) * list (svar Tbool))%type)
-  : forall sv vs (G : list (sigT (fun t : vartype => (interp_type t * (interp_type t * SymbolicExpr))%type))) (xs : mapping),
-    (forall t x1 sv x2, In (existT _ t (x1, (x2, sv))) G -> x1 = x2)
-    -> (forall t x1 sv x2,
-           In (existT _ t (x1, (x2, sv))) G -> symbolic_eval vs sv = Some x1)
-    -> (forall t x sv, lookup (var:=var) t sv xs = Some x -> In (existT _ t (x, (x, sv))) G)
-    -> forall t, match lookup (var:=var) t sv xs with
-                 | Some x' => symbolic_eval vs sv = Some x' /\ In (existT _ t (x', (x', sv))) G
-                 | None => True
-                 end.
-Proof.
-  induction xs;
-    repeat first [ congruence
-                 | solve [ trivial ]
-                 | progress intros
-                 | progress subst
-                 | progress simpl in *
-                 | progress break_match
-                 | progress inversion_option
-                 | progress specialize_vartype
-                 | solve [ eauto ] ].
-Qed.
-
-(*
-Local Ltac SymbolicExpr_beq_to_eq :=
-  repeat match goal with
-         | [ H : SymbolicExpr_beq _ _ = true |- _ ] => apply internal_SymbolicExpr_dec_bl in H
-         | [ H : context[SymbolicExpr_beq ?x ?x] |- _ ]
-           => rewrite (@internal_SymbolicExpr_dec_lb x x eq_refl) in H
-         end.
-Lemma wf_good_lookup t G s xs b
-      (H : wf_context_mapping_good G xs)
-  : lookup (var:=interp_type) t s xs = Some b
-    -> option_map Output.interp (symbolic_eval xs s) = Some b.
-Proof.
-  destruct xs as [ls0 ls1], t; simpl in *;
-    first [ revert dependent ls0; induction ls1 as [|?? IHxs]
-          | revert dependent ls1; induction ls0 as [|?? IHxs] ];
-    repeat match goal with
-           | _ => congruence
-           | _ => progress simpl
-           | _ => progress break_match
-           | _ => progress intros
-           | _ => progress congruence_option
-           | _ => progress SymbolicExpr_beq_to_eq
-           | _ => progress subst
-           end.
-Admitted.
-
-Local Ltac apply_lookup_good :=
-  repeat match goal with
-         | [ H : lookup' _ _ = Some _ |- _ ]
-           => first [ eapply (@wf_good_lookup Tbool) in H; [ | eassumption ]
-                    | eapply (@wf_good_lookup TW) in H; [ | eassumption ] ]
-         end.
-
-Lemma wf_context_mapping_good_In_sym_eval_eq t G xs x b x'
-      (H : wf_context_mapping_good G xs)
-      (HIn : In (existT _ t (x, x')) G)
-  : option_map Output.interp (symbolic_eval (t := t) xs (snd x')) = Some b
-    -> b = x.
-Proof.
-Admitted.
-
-Lemma wf_good_lookup_None_In t G xs x x'
-      (H : wf_context_mapping_good G xs)
-      (HIn : In (existT _ t (x, x')) G)
-  : lookup (var:=interp_type) t (snd x') xs = None
-    -> fst x' = x.
-Proof.
-  destruct xs as [ls0 ls1], t; simpl in *;
-    first [ revert dependent ls0; induction ls1 as [|?? IHxs]
-          | revert dependent ls1; induction ls0 as [|?? IHxs] ];
-    repeat match goal with
-           | _ => congruence
-           | _ => progress simpl
-           | _ => progress break_match
-           | _ => progress intros
-           | _ => progress congruence_option
-           | _ => progress SymbolicExpr_beq_to_eq
-           | _ => progress subst
-           end.
-Admitted.
-
-(*Local Ltac use_wf_context_mapping_good_In_sym_eval_eq
-  := repeat match goal with
-            | [ H : option_map Output.interp (symbolic_eval (t := Tflat (Tconst (Tvar ?t))) ?xs (snd ?x')) = Some ?b |- _]
-              => eapply (@wf_context_mapping_good_In_sym_eval_eq t _ xs _ b x') in H; [ | eassumption | eassumption ]
-            end.
-
-Lemma wf_to_interp_arg t G x x' xs
-      (wf : Output.wf_arg G x x')
-      (Hgood : wf_context_mapping_good G xs)
-  : Output.interp_arg (fst (cseArg x' xs)) = Output.interp_arg (t := t) x.
-Proof.
-  revert dependent xs; induction wf;
-    repeat match goal with
-           | _ => reflexivity
-           | _ => progress intros
-           | _ => progress subst
-           | _ => progress simpl in *
-           | _ => progress break_match
-           | _ => progress congruence_option
-           | _ => progress apply_lookup_good
-           | _ => progress use_wf_context_mapping_good_In_sym_eval_eq
-           | _ => progress unfold cseExprHelper1, cseExprHelper2 in *
-           end.
-lazymatch goal with
-            | [ H : option_map Output.interp (symbolic_eval (t := Tflat (Tconst (Tvar ?t))) ?xs (snd ?x')) = Some ?b |- _]
-              => eapply (@wf_context_mapping_good_In_sym_eval_eq t _ xs _ b x') in H
-end.
-eapply wf_context_mapping_good_In_sym_eval_eq in Heqo.
-eappply
-
-Lemma wf_context_mapping_good_unop G t (op : nop 1 1 t TW) xs s w
-      (e : @Output.arg interp_type t)
-      (e' : @Output.arg (fun t' => interp_type t' * SymbolicExpr)%type t)
-      (H : wf_context_mapping_good G xs)
-      (Heq : snd (cseArg (var:=interp_type) e' xs) = Some s)
-      (Hlookup : lookup (var:=interp_type) TW (SUnOp (cseOp op) s) xs = Some w)
-      (wf : Output.wf_arg G e e')
-  : wf_context_mapping_good
-      (existT _ _ (interp_nop op (Output.interp_arg e), (w, SUnOp (cseOp op) s)) :: G) xs.
-Proof.
-  revert dependent s.
-  revert dependent w.
-  revert H.
-  induction wf;
-    repeat match goal with
-           | _ => progress intros
-           | _ => progress subst
-           | _ => progress simpl in *
-           | _ => progress break_match
-           | _ => progress congruence_option
-           | _ => progress unfold cseExprHelper1, cseExprHelper2 in *
-           end.
-Admitted.
-(*Lemma wf_context_mapping_good_unop' G t (op : nop 1 1 t TW) xs s w
-      (e : @Output.arg interp_type t)
-      (e' : @Output.arg (fun t' => interp_type t' * SymbolicExpr)%type t)
-      (H : wf_context_mapping_good G xs)
-      (Heq : snd (cseArg (var:=interp_type) e' xs) = Some s)
-      (Hlookup : lookup (var:=interp_type) TW (SUnOp (cseOp op) s) xs = None)
-      (wf : Output.wf_arg G e e')
-  : wf_context_mapping_good
-      (existT _ _ (interp_nop op (Output.interp_arg e), (w, SUnOp (cseOp op) s)) :: G) xs.
-Proof.
-  wf_context_mapping_good
-    (existT
-       (fun t : vartype =>
-        (match t with
-         | Tbool => bool
-         | TW => fancy_machine.W
-         end * (match t with
-                | Tbool => bool
-                | TW => fancy_machine.W
-                end * SymbolicExpr))%type) TW
-       (interp_nop op (Output.interp_arg e1),
-       (interp_nop op (Output.interp_arg (fst (cseArg e1' xs))), SUnOp (cseOp op) s)) :: G)
-    ((interp_nop op (Output.interp_arg (fst (cseArg e1' xs))), SUnOp (cseOp op) s) :: fst xs, snd xs)
-*)*)*)
-
-Definition wf_context_mapping_good
-           (var := interp_type)
-           (svar := fun t => (var t * SymbolicExpr)%type)
-           (mapping := (list (svar TW) * list (svar Tbool))%type)
-  : list (sigT (fun t : vartype => (interp_type t * (interp_type t * SymbolicExpr))%type))
-    -> mapping
-    -> Prop
-  := fun G xs
-     => (forall t x1 sv x2, In (existT _ t (x1, (x2, sv))) G -> x1 = x2)
-        /\ (forall t x1 sv x2,
-               In (existT _ t (x1, (x2, sv))) G -> symbolic_eval xs sv = Some x1)
-        /\ (forall t x sv, lookup (var:=var) t sv xs = Some x -> In (existT _ t (x, (x, sv))) G).
-
-(*Lemma wf_context_mapping_good_cons g G xs
-  : wf_context_mapping_good (g :: G) xs
-    <-> (let '(x1, (x2, sv)) := eta3' (projT2 g) in
-         x1 = x2
-         /\ symbolic_eval xs sv = Some x1
-         /\ ((forall t, lookup (var:=interp_type) t sv xs = None) \/ In g G)
-         /\ wf_context_mapping_good G xs).
-Proof.
-  destruct g as [? [? [? ?] ] ]; simpl.
-  unfold wf_context_mapping_good; simpl;
-    repeat intuition (subst || inversion_sigma || inversion_prod || simpl in * || eauto || specialize_vartype).
-  destruct x.
-  repeat match goal with
-         | [ x : _, H' : forall y, _ |- _ ] => unique pose proof (H' x)
-         end.
-  repeat match goal with
-         | [ H : None = Some _ -> _ |- _ ] => clear H
-         | [ H : ?x = ?x -> _ |- _ ] => specialize (H eq_refl)
-         | [ H : @lookup' ?a ?b ?c ?d = Some _ -> _ |- _ ]
-           => destruct (@lookup' a b c d) eqn:?
-         end.
-
-
-         end.
-  { repeat match goal with
-         | [ H : or _ _ |- _ ] => destruct H
-         end.
-  specialize_all_ways.
-Qed.
-
-Definition wf_context_mapping_good_cons1 g G xs
-  := proj2 (wf_context_mapping_good_cons g G xs).
-
-Lemma cseArg_correct {t} (x1 : @Output.arg interp_type t) (x2 : @Output.arg (fun t : vartype => (interp_type t * SymbolicExpr)%type) t) G (wf:Output.wf_arg G x1 x2) xs :
-  wf_context_mapping_good G xs ->
-    Output.pointwise_eq_interp (t := t) (Output.interp_arg (fst (cseArg x2 xs))) (Output.interp_arg x1).
-Proof.
-  revert dependent xs; induction wf;
-    repeat match goal with
-           | _ => congruence
-           | _ => progress intros
-           | _ => progress subst
-           | _ => progress simpl in *
-           | _ => progress break_match
-           | _ => progress inversion_option
-           | _ => progress unfold cseExprHelper1, cseExprHelper2 in *
-           end.
-
-  t : flat_type
-  x : Output.arg t
-  x' : Output.arg t
-  H0 : Output.wf_arg G x x'
-  xs : list (fancy_machine.W * SymbolicExpr) * list (bool * SymbolicExpr)
-  H1 : wf_context_mapping_good G xs
-  ============================
-  Output.interp_arg (fst (cseArg x' xs)) = Output.interp_arg x
-
-
-Lemma cse'_correct {t} (e1 : @Output.expr interp_type t) (e2 : @Output.expr (fun t : vartype => (interp_type t * SymbolicExpr)%type) t) G (wf:Output.wf G e1 e2) xs :
-  wf_context_mapping_good G xs ->
-    Output.pointwise_eq_interp (t := t) (Output.interp (cseExpr' e2 xs)) (Output.interp e1).
-Proof.
-  revert dependent xs.
-  induction wf;
-    repeat match goal with
-           | _ => congruence
-           | _ => progress intros
-           | _ => progress subst
-           | _ => progress simpl in *
-           | _ => progress break_match
-           | _ => progress inversion_option
-           | _ => progress unfold cseExprHelper1, cseExprHelper2 in *
-           end.
-  { match goal with
-    | [ H : _ |- _ ] => apply H, wf_context_mapping_good_cons1; simpl
-    end.
-    split; eauto.
-    admit. }
-  { match goal with
-    | [ H : _ |- _ ] => apply H, wf_context_mapping_good_cons1; simpl
-    end.
-    admit. }
-  { match goal with
-    | [ H : _ |- _ ] => apply H, wf_context_mapping_good_cons1; simpl
-    end.
-    admit. }
-  { match goal with
-    | [ H : _ |- _ ] => apply H, wf_context_mapping_good_cons1; simpl
-    end.
-    admit. }
-  { match goal with
-    | [ H : _ |- _ ] => apply H, wf_context_mapping_good_cons1; simpl
-    end.
-    admit. }
-  { match goal with
-    | [ H : _ |- _ ] => apply H, wf_context_mapping_good_cons1; simpl
-    end.
-    admit. }
-  { match goal with
-    | [ H : _ |- _ ] => apply H, wf_context_mapping_good_cons1; simpl
-    end.
-    admit. }
-  { match goal with
-    | [ H : _ |- _ ] => apply H, wf_context_mapping_good_cons1; simpl
-    end.
-    admit. }
-  { match goal with
-    | [ H : _ |- _ ] => apply H, wf_context_mapping_good_cons1; simpl
-    end.
-    admit. }
-  { match goal with
-    | [ H : _ |- _ ] => apply H, wf_context_mapping_good_cons1; simpl
-    end.
-    admit. }
-  { match goal with
-    | [ H : _ |- _ ] => apply H, wf_context_mapping_good_cons1; simpl
-    end.
-    admit. }
-  { match goal with
-    | [ H : _ |- _ ] => apply H, wf_context_mapping_good_cons1; simpl
-    end.
-    admit. }
-  { match goal with
-    | [ H : _ |- _ ] => apply H, wf_context_mapping_good_cons1; simpl
-    end.
-    admit. }
-  { match goal with
-    | [ H : _ |- _ ] => apply H, wf_context_mapping_good_cons1; simpl
-    end.
-    admit. }
-  { match goal with
-    | [ H : _ |- _ ] => apply H, wf_context_mapping_good_cons1; simpl
-    end.
-    admit. }
-  { match goal with
-    | [ H : _ |- _ ] => apply H, wf_context_mapping_good_cons1; simpl
-    end.
-    admit. }
-  { match goal with
-    | [ H : _ |- _ ] => apply H, wf_context_mapping_good_cons1; simpl
-    end.
-    admit. }
-  { match goal with
-    | [ H : _ |- _ ] => apply H, wf_context_mapping_good_cons1; simpl
-    end.
-    admit. }
-  { match goal with
-    | [ H : _ |- _ ] => apply H, wf_context_mapping_good_cons1; simpl
-    end.
-    admit. }
-  { match goal with
-    | [ H : _ |- _ ] => apply H, wf_context_mapping_good_cons1; simpl
-    end.
-    admit. }
-  {
-match goal with
-    | [ H : _ |- _ ] => apply H, wf_context_mapping_good_cons1; simpl
-    end.
-    admit. }
-  { apply H2, wf_context_mapping_good_cons1; simpl.
-    admit. }
-  {
-apply H2, wf_context_mapping_good_cons1; simpl.
-    admit. }
-    a
-    unfold wf_context_mapping_good in *.
-    simpl.
-    intros.
-
-    [ apply H2
-    | apply H2
-    | try apply H2
-    | try apply H2
-    | try apply H2
-    | try apply H2
-    | try apply H2
-    | try apply H2
-    | try apply H2
-    | try apply H2
-    | try apply H2
-    | try apply H2
-    | try apply H2
-    | try apply H2
-    | try apply H2
-    | try apply H2
-    | try apply H2
-    | try apply H2
-    | try apply H2
-    | ].
-  Focus 20.
-  {
-Set Printing Implicit.
-  { apply H2.
-
-
-pose @symbolic_eval.
-cbv beta in *.
-Set Printing All.
-
-simpl.
-  induction wf;
-    repeat match goal with
-    | [HIn:In ?x ?l, HForall:Forall _ ?l |- _ ] =>
-      (pose proof (proj1 (Forall_forall _ _) HForall _ HIn); clear HIn)
-    | [ H : Output.match_arg_Prod _ = (_, _) |- _ ] =>
-      apply Output.match_arg_Prod_correct in H
-    | [ H : Output.Pair _ _ = Output.Pair _ _ |- _ ] =>
-      apply Output.Pair_eq in H
-    | [ H : (_, _) = (_, _) |- _ ] => inversion H; clear H
-    | _ => progress intros
-    | _ => progress simpl in *
-    | _ => progress subst
-    | _ => progress specialize_by assumption
-    | _ => progress break_match
-    | _ => rewrite !Output.interp_under_lets
-    | _ => rewrite !Output.interp_arg_uninterp_arg
-    | _ => progress erewrite_hyp !*
-    | _ => apply Forall_cons
-    | _ => solve [intuition (congruence || eauto)]
-    end.
-Qed.
-
-Lemma Compile_correct {_: Evaluable Z} {t} (E:Input.Expr t) (WfE:Input.Wf E) :
-  Output.Interp (Compile E) = Input.Interp E.
-Proof. eapply compile_correct; eauto. Qed.
- *)
-
+  Definition rexpression_simple := Eval vm_compute in CSE ops (InlineConst (Linearize rexpression)).
+End reflected.
 
 Section syn.
-  Context {var : vartype -> Type}.
+  Context {var : base_type -> Type}.
   Inductive syntax :=
   | RegPInv
   | RegMod
   | RegZero
+  | cConstZ : Z -> syntax
+  | cConstBool : bool -> syntax
   | cLowerHalf : syntax -> syntax
   | cUpperHalf : syntax -> syntax
   | cLeftShifted : syntax -> Z -> syntax
@@ -1693,6 +198,101 @@ Section syn.
 End syn.
 
 Definition Syntax := forall var, @syntax var.
+
+Section assemble.
+  Context (ops : fancy_machine.instructions (2 * 128)).
+
+  Section with_var.
+    Context {var : base_type -> Type}.
+
+    Fixpoint assemble_syntax_const
+             {t}
+      : interp_flat_type_gen (interp_base_type _) t -> @syntax var
+      := match t return interp_flat_type_gen (interp_base_type _) t -> @syntax var with
+         | Tbase TZ => cConstZ
+         | Tbase Tbool => cConstBool
+         | Tbase t => fun _ => cINVALID t
+         | Prod A B => fun xy => cPair (@assemble_syntax_const A (fst xy))
+                                       (@assemble_syntax_const B (snd xy))
+         end.
+
+    Definition assemble_syntaxf_step
+               (assemble_syntaxf : forall {t} (v : @Syntax.exprf base_type (interp_base_type _) op (fun _ => @syntax var) t), @syntax var)
+               {t} (v : @Syntax.exprf base_type (interp_base_type _) op (fun _ => @syntax var) t) : @syntax var.
+    Proof.
+      refine match v with
+             | Syntax.Const t x => assemble_syntax_const x
+             | Syntax.Var _ x => x
+             | Syntax.Op _ _ op args => _
+             | Syntax.Let _ ex _ eC
+               => cBind (@assemble_syntaxf _ ex) (fun x => @assemble_syntaxf _ (eC _))
+             | Syntax.Pair _ ex _ ey
+               => cPair (@assemble_syntaxf _ ex) (@assemble_syntaxf _ ey)
+             end.
+Focus 2.
+  refine match v with
+         | Output.LetUnop _ op x0 _ b
+           => let x0' := assemble_arg x0 in
+              match op with
+              | OPldi => @assemble_syntax var _ (b x0')
+              | _ => cINVALID op
+              end
+         | Output.LetBinop _ _ op x0 x1 _ b
+           => let x0' : @syntax var := assemble_arg x0 in
+              let x1' : @syntax var := assemble_arg x1 in
+              let default := fun s => cBind s (fun v => @assemble_syntax var _ (b (cVar v))) in
+              match op, x1 return @syntax var with
+              | OPshl, Output.Const TZ x1'
+                => @assemble_syntax var _ (b (cLeftShifted x0' x1'))
+              | OPshr, Output.Const TZ x1'
+                => @assemble_syntax var _ (b (cRightShifted x0' x1'))
+              | OPmulhwll, _
+                => default (cMul128 (cLowerHalf x0') (cLowerHalf x1'))
+              | OPmulhwhl, _
+                => default (cMul128 (cUpperHalf x0') (cLowerHalf x1'))
+              | OPmulhwhh, _
+                => default (cMul128 (cUpperHalf x0') (cUpperHalf x1'))
+              | _, _ => default (cINVALID op)
+              end
+         | Output.LetTrinop _ _ _ op x0 x1 x2 _ b
+           => let x0' : @syntax var := assemble_arg x0 in
+              let x1' : @syntax var := assemble_arg x1 in
+              let x2' : @syntax var := assemble_arg x2 in
+              cBind (match op, x0', x2', x2 return @syntax var with
+                     | OPadc, _, _, Output.Const Tbool false
+                       => cAdd x0' x1'
+                     | OPadc, _, cVarC x2', _
+                       => cAddc x2' x0' x1'
+                     | OPsubc, _, _, Output.Const Tbool false
+                       => cSub x0' x1'
+                     | OPselc, cVarC x0', _, _
+                       => cSelc x0' x1' x2'
+                     | OPaddm, _, RegMod, _
+                       => cAddm x0' x1'
+                     | _, _, _, _ => cINVALID op
+                     end)
+                    (fun v => @assemble_syntax var _ (b (cVar v)))
+         | Output.LetTrinop2Ret _ _ _ op x0 x1 x2 _ b
+           => let x0' : @syntax var := assemble_arg x0 in
+              let x1' : @syntax var := assemble_arg x1 in
+              let x2' : @syntax var := assemble_arg x2 in
+              cBindCarry (match op, x0', x2', x2 return @syntax var with
+                          | OPadc, _, _, Output.Const Tbool false
+                            => cAdd x0' x1'
+                          | OPadc, _, cVarC x2', _
+                            => cAddc x2' x0' x1'
+                          | OPsubc, _, _, Output.Const Tbool false
+                            => cSub x0' x1'
+                          | _, _, _, _ => cINVALID op
+                          end)
+                         (fun c v => @assemble_syntax var _ (b (cVarC c) (cVar v)))
+         | Output.Return _ x => @assemble_arg var _ x
+         | Output.Abs TW d f => cAbs (fun x : var TW => @assemble_syntax var _ (f (cVar x)))
+         | Output.Abs s _ _ => cINVALID s
+         end.
+  exact (fun _ => unit).
+Defined.
+
 
 Fixpoint assemble_arg {var} {t} (v : @Output.arg (fun _ => @syntax var) t) : @syntax var
   := match v with
